SSA/Projects/DCE/DCE.lean
@@ -8,80 +8,98 @@ open Ctxt (Var Valuation Hom)
 
 
 /-- Delete a variable from a list. -/
-def Ctxt.delete (Γ : Ctxt Ty) (v : Γ.Var α) : Ctxt Ty :=
-  ⟨Γ.toList.eraseIdx v.val⟩
+def Ctxt.delete (Γ : Ctxt Ty) (vs : HVector Γ.Var α) : Ctxt Ty :=
+  ⟨vs.foldl (fun _ Γ v => Γ.eraseIdx v.val) Γ.toList⟩
 
-@[simp] theorem Ctxt.delete_snoc_toSnoc {Γ : Ctxt Ty} {v : Γ.Var t} :
-    (Γ.snoc u).delete (v.toSnoc) = (Γ.delete v).snoc u := rfl
+-- @[simp] theorem Ctxt.delete_snoc_toSnoc {Γ : Ctxt Ty} {v : Γ.Var t} :
+--     (Γ.snoc u).delete (v.toSnoc) = (Γ.delete v).snoc u := rfl
 
-def Hom.delete {Γ : Ctxt Ty} (delv : Γ.Var t) : Hom (Γ.delete delv) Γ :=
-  fun t' v =>
-    let idx :=
-      if v.val < delv.val then
-        v.val
-      else
-        v.val + 1
-    ⟨idx, by
-      unfold idx
-      split_ifs with h_val
-      <;> simpa [Ctxt.delete, List.getElem?_eraseIdx, h_val] using v.prop
-    ⟩
+@[simp] theorem Ctxt.delete_append_appendInl {Γ : Ctxt Ty} {us : List Ty}
+    {vs : HVector Γ.Var ts} :
+    (Γ ++ us).delete (vs.map (fun _ v => v.appendInl)) = (Γ.delete vs) ++ us := by
+  sorry
 
-@[simp] lemma Hom.delete_toSnoc_toSnoc {Γ : Ctxt Ty}
-    {delv : Γ.Var t} {v : (Γ.delete delv).Var t'} :
-    Hom.delete (delv.toSnoc : (Γ.snoc u).Var t) v.toSnoc = (Hom.delete delv v).toSnoc := by
-  simp only [delete, Var.val_toSnoc, add_lt_add_iff_right]
-  split <;> rfl
+def Hom.delete {Γ : Ctxt Ty} (delv : HVector Γ.Var ts) : Hom (Γ.delete delv) Γ :=
+  sorry
+  -- fun t' v =>
+  --   let idx :=
+  --     if v.val < delv.val then
+  --       v.val
+  --     else
+  --       v.val + 1
+  --   ⟨idx, by
+  --     unfold idx
+  --     split_ifs with h_val
+  --     <;> simpa [Ctxt.delete, List.getElem?_eraseIdx, h_val] using v.prop
+  --   ⟩
+
+-- @[simp] lemma Hom.delete_toSnoc_toSnoc {Γ : Ctxt Ty}
+--     {delv : HVector Γ.Var ts} {v : (Γ.delete delv).Var t'} :
+--     Hom.delete (delv.toSnoc : (Γ.snoc u).Var t) v.toSnoc = (Hom.delete delv v).toSnoc := by
+--   simp only [delete, Var.val_toSnoc, add_lt_add_iff_right]
+--   split <;> rfl
 
 /-- Witness that Γ' is Γ without v -/
-def Deleted {α : Ty} (Γ: Ctxt Ty) (v : Γ.Var α) (Γ' : Ctxt Ty) : Prop :=
-  Γ' = Γ.delete v
+def Deleted {α : List Ty} (Γ: Ctxt Ty) (vs : HVector Γ.Var α) (Γ' : Ctxt Ty) : Prop :=
+  Γ' = Γ.delete vs
 
-/-- build a `Deleted` for a `(Γ.snoc α) → Γ`-/
-def Deleted.deleteSnoc (Γ : Ctxt Ty) (α : Ty) : Deleted (Γ.snoc α) (Ctxt.Var.last Γ α) Γ := rfl
+def Var.varsOfType {Γ : Ctxt Ty} (ts : List Ty) : HVector (Var <| Γ ++ ts) ts :=
+  (HVector.ofFn (Var ⟨ts⟩) _ Var.ofFin)
+    |>.map (fun _ v => v.appendInr)
+
+/-- build a `Deleted` for a `(Γ ++ αs) → Γ`-/
+def Deleted.deleteAppend (Γ : Ctxt Ty) (αs : List Ty) :
+    Deleted (Γ ++ αs) (Var.varsOfType αs) Γ :=
+  sorry -- rfl
 
 
-/-- snoc an `ω` to both the input and output contexts of `Deleted Γ v Γ'` -/
-def Deleted.snoc {α : Ty} {Γ : Ctxt Ty} {v : Γ.Var α}
-    (DEL : Deleted Γ v Γ') (ω : Ty) :
-    Deleted (Γ.snoc ω) v.toSnoc (Γ'.snoc ω) := by
+/-- append an `ωs` to both the input and output contexts of `Deleted Γ v Γ'` -/
+def Deleted.append {αs} {Γ : Ctxt Ty} {vs : HVector Γ.Var αs}
+    (DEL : Deleted Γ vs Γ') (ω : List Ty) :
+    Deleted (Γ ++ ωs) (vs.map fun _ v => v.appendInl) (Γ' ++ ωs) := by
+  stop
   simp only [Deleted, Ctxt.delete, Ctxt.Var.val_toSnoc] at DEL ⊢
   subst DEL
   rfl
 
 def Deleted.toHom (h : Deleted Γ v Γ') : Γ'.Hom Γ :=
-  h ▸ Hom.delete _
+  sorry -- h ▸ Hom.delete _
 
-@[simp] lemma Deleted.toHom_snoc {Γ Γ' : Ctxt Ty} {v : Γ.Var t}
-    (DEL : Deleted (Γ.snoc u) v.toSnoc (Γ'.snoc u)) :
-    DEL.toHom =
-      have DEL' : Deleted Γ v Γ' := by
+@[simp] lemma Deleted.toHom_append {Γ Γ' : Ctxt Ty} {vs : HVector Γ.Var ts}
+    (DEL : Deleted (Γ ++ us) (vs.map fun _ v => v.appendInl) (Γ' ++ us)) :
+    DEL.toHom
+    = have DEL' : Deleted Γ vs Γ' := by
         rcases Γ'
-        simp only [Deleted, Ctxt.delete_snoc_toSnoc] at DEL ⊢
+        simp only [Deleted, Ctxt.delete_append_appendInl] at DEL ⊢
         injection DEL
         simp_all [Ctxt.delete]
-      DEL'.toHom.snocMap := by
-  have DEL' : Deleted Γ v Γ' := by
+      DEL'.toHom.append := by
+  have DEL' : Deleted Γ vs Γ' := by
     rcases Γ'
-    simp only [Deleted, Ctxt.delete_snoc_toSnoc] at DEL ⊢
+    simp only [Deleted, Ctxt.delete_append_appendInl] at DEL ⊢
     injection DEL
     simp_all [Ctxt.delete]
   subst DEL'
   funext t v;
+  stop
   simp only [Deleted.toHom]
   cases v
   · simp
   · simp [Hom.delete]
 
-@[simp] lemma Deleted.toHom_last (DEL : Deleted (Γ.snoc u) (Var.last _ _) Γ) :
-    DEL.toHom = Hom.id.snocRight := rfl
+@[simp] lemma Deleted.toHom_last (DEL : Deleted (Γ ++ us) (Var.varsOfType us) Γ) :
+    DEL.toHom = Hom.id.appendCodomain := by
+  sorry
 
 /-! ## tryDelete? -/
 
 /-- Given  `Γ' := Γ/delv`, transport a variable from `Γ` to `Γ', if `v ≠ delv`. -/
-def Var.tryDelete? [TyDenote Ty] {Γ Γ' : Ctxt Ty} {delv : Γ.Var α}
-  (DEL : Deleted Γ delv Γ') (v : Γ.Var β) :
-    Option { v' : Γ'.Var β // v = (DEL.toHom) v' } :=
+def Var.tryDelete? [TyDenote Ty] {Γ Γ' : Ctxt Ty} {delv : HVector Γ.Var α}
+  (DEL : Deleted Γ delv Γ') (vs : HVector Γ.Var β) :
+    Option { v' : HVector Γ'.Var β // vs = v'.map DEL.toHom } :=
+  by
+  stop
+  exact
   if h_val_eq : v.val = delv.val then
     none -- if it's the deleted variable, then return nothing.
   else
@@ -108,23 +126,24 @@ namespace DCE
 
 variable {d : Dialect} [TyDenote d.Ty]
 
-/-- Try to delete the variable from the argument list.
-  Succeeds if variable does not occur in the argument list.
-  Fails otherwise. -/
-def arglistDeleteVar? {Γ: Ctxt d.Ty} {delv : Γ.Var α} {Γ' : Ctxt d.Ty} {ts : List d.Ty}
-  (DEL : Deleted Γ delv Γ')
-  (as : HVector (Ctxt.Var Γ) <| ts) :
-  Option
-    { as' : HVector (Ctxt.Var Γ') <| ts // as = as'.map DEL.toHom } :=
-  match as with
-  | .nil => .some ⟨.nil, by rfl⟩
-  | .cons a as =>
-    match Var.tryDelete? DEL a with
-    | .none => .none
-    | .some ⟨a', ha'⟩ =>
-      match arglistDeleteVar? DEL as with
-      | .none => .none
-      | .some ⟨as', has'⟩ => .some ⟨.cons a' as', by simp [HVector.map_cons, *]⟩
+-- /-- Try to delete the variable from the argument list.
+--   Succeeds if variable does not occur in the argument list.
+--   Fails otherwise. -/
+-- def arglistDeleteVar? {Γ: Ctxt d.Ty} {delv : HVector Γ.Var us} {Γ' : Ctxt d.Ty} {ts : List d.Ty}
+--     (DEL : Deleted Γ delv Γ')
+--     (as : HVector Γ.Var ts) :
+--     Option { as' : HVector (Ctxt.Var Γ') <| ts // as = as'.map DEL.toHom } :=
+--   Var.tryDelete? DEL as
+
+  -- match as with
+  -- | .nil => .some ⟨.nil, by rfl⟩
+  -- | .cons a as =>
+  --   match Var.tryDelete? DEL a with
+  --   | .none => .none
+  --   | .some ⟨a', ha'⟩ =>
+  --     match arglistDeleteVar? DEL as with
+  --     | .none => .none
+  --     | .some ⟨as', has'⟩ => .some ⟨.cons a' as', by simp [HVector.map_cons, *]⟩
 
 variable [DialectSignature d] [DialectDenote d] [Monad d.m] [LawfulMonad d.m]
 
@@ -134,7 +153,7 @@ def Expr.deleteVar? (DEL : Deleted Γ delv Γ') (e: Expr d Γ .pure t) :
     e.denoteOp V = e'.denoteOp (V.comap DEL.toHom) } :=
   match e with
   | .mk op ty_eq eff_le args regArgs => do
-    let args' ← arglistDeleteVar? DEL args
+    let args' ← Var.tryDelete? DEL args
     some ⟨.mk op ty_eq eff_le args' regArgs, by
       obtain ⟨ args', rfl ⟩ := args'
       intros V
@@ -143,15 +162,19 @@ def Expr.deleteVar? (DEL : Deleted Γ delv Γ') (e: Expr d Γ .pure t) :
     ⟩
 
 /-- Delete a variable from an Com. -/
-def Com.deleteVar? (DEL : Deleted Γ delv Γ') (com : Com d Γ .pure t) :
-  Option { com' : Com d Γ' .pure t // ∀ (V : Γ.Valuation),
-    com.denote V = com'.denote (V.comap DEL.toHom) } :=
+def Com.deleteVar? (DEL : Deleted Γ delv Γ')
+    (com : Com d Γ .pure ts) :
+    Option { com' : Com d Γ' .pure ts // ∀ (V : Γ.Valuation),
+      com.denote V = com'.denote (V.comap DEL.toHom) } :=
   match com with
-  | .ret v => do
-    let ⟨v, hv⟩ ← Var.tryDelete? DEL v
-    return ⟨.ret v, by simp [hv]⟩
-  | .var (α := ω) e body => do
-    let ⟨body', hbody'⟩ ← Com.deleteVar? (DEL.snoc _) body
+  | .ret vs => do
+    let ⟨vs, hv⟩ ← Var.tryDelete? DEL vs
+    return ⟨.ret vs, by
+      intro V
+      simp [hv, HVector.map_map]; rfl
+    ⟩
+  | .var (ty := ω) e body => do
+    let ⟨body', hbody'⟩ ← Com.deleteVar? (DEL.append ω) body
     let ⟨e', he'⟩ ← Expr.deleteVar? DEL e
     .some ⟨.var e' body', by
       intros V
@@ -165,12 +188,12 @@ and ensure that Lean does not freak out on us, since it's indeed unclear to Lean
 that the output type of `dce` is always inhabited.
 -/
 def DCEType [DialectSignature d] [DialectDenote d] {Γ : Ctxt d.Ty}
-    {t : d.Ty} (com : Com d Γ .pure t) : Type :=
+    {t} (com : Com d Γ .pure t) : Type :=
   Σ (Γ' : Ctxt d.Ty) (hom: Hom Γ' Γ),
     { com' : Com d Γ' .pure t //  ∀ (V : Γ.Valuation), com.denote V = com'.denote (V.comap hom)}
 
 /-- Show that DCEType in inhabited. -/
-instance [SIG : DialectSignature d] [DENOTE : DialectDenote d] {Γ : Ctxt d.Ty} {t : d.Ty}
+instance [SIG : DialectSignature d] [DENOTE : DialectDenote d] {Γ : Ctxt d.Ty} {t}
     (com : Com d Γ .pure t) : Inhabited (DCEType com) where
   default :=
     ⟨Γ, Hom.id, com, by intros V; rfl⟩
@@ -181,7 +204,7 @@ defined by the `let` in the body/ Note that this is `O(n^2)`, for an easy
 proofs, as it is written as a forward pass.  The fast `O(n)` version is a
 backward pass.
 -/
-partial def dce_ {Γ : Ctxt d.Ty} {t : d.Ty}
+partial def dce_ {Γ : Ctxt d.Ty} {t}
     (com : Com d Γ .pure t) : DCEType com :=
   match HCOM: com with
   | .ret v => -- If we have a `ret`, return it.
@@ -190,17 +213,17 @@ partial def dce_ {Γ : Ctxt d.Ty} {t : d.Ty}
       unfold Ctxt.Valuation.comap
       simp
       ⟩⟩
-  | .var (α := α) e body =>
-    let DEL := Deleted.deleteSnoc Γ α
+  | .var (ty := tys) e body =>
+    let DEL := Deleted.deleteAppend Γ tys
     -- Try to delete the variable α in the body.
     match Com.deleteVar? DEL body with
     | .none => -- we don't succeed, so DCE the child, and rebuild the same `let` binding.
       let ⟨Γ', hom', ⟨body', hbody'⟩⟩
-        : Σ (Γ' : Ctxt d.Ty) (hom: Hom Γ' (Ctxt.snoc Γ α)),
-        { body' : Com d Γ' .pure t //  ∀ (V : (Γ.snoc α).Valuation),
+        : Σ (Γ' : Ctxt d.Ty) (hom: Hom Γ' (Γ ++ tys)),
+        { body' : Com d Γ' .pure t //  ∀ (V : (Γ ++ tys).Valuation),
         body.denote V = body'.denote (V.comap hom)} :=
         (dce_ body)
-      let com' := Com.var (α := α) e (body'.changeVars hom')
+      let com' := Com.var e (body'.changeVars hom')
       ⟨Γ, Hom.id, com', by
         intros V
         apply Id.ext
@@ -233,14 +256,14 @@ partial def dce_ {Γ : Ctxt d.Ty} {t : d.Ty}
 /-- This is the real entrypoint to `dce` which unfolds the type of `dce_`, where
 we play the `DCEType` trick to convince Lean that the output type is in fact
 inhabited. -/
-def dce {Γ : Ctxt d.Ty} {t : d.Ty} (com : Com d Γ .pure t) :
+def dce {Γ : Ctxt d.Ty} {t} (com : Com d Γ .pure t) :
   Σ (Γ' : Ctxt d.Ty) (hom: Hom Γ' Γ),
     { com' : Com d Γ' .pure t //  ∀ (V : Γ.Valuation), com.denote V = com'.denote (V.comap hom)} :=
   dce_ com
 
 /-- A version of DCE that returns an output program with the same context. It uses the context
    morphism of `dce` to adapt the result of DCE to work with the original context -/
-def dce' {Γ : Ctxt d.Ty} {t : d.Ty}
+def dce' {Γ : Ctxt d.Ty} {t}
     (com : Com d Γ .pure t) :
     { com' : Com d Γ .pure t //  ∀ (V : Γ.Valuation), com.denote V = com'.denote V} :=
   let ⟨ Γ', hom, com', hcom'⟩ := dce_ com
@@ -272,18 +295,18 @@ abbrev Ex : Dialect where
 
 instance : DialectSignature Ex where
   signature
-    | .add    => ⟨[.nat, .nat], [], .nat, .pure⟩
-    | .beq    => ⟨[.nat, .nat], [], .bool, .pure⟩
-    | .cst _  => ⟨[], [], .nat, .pure⟩
+    | .add    => ⟨[.nat, .nat], [], [.nat], .pure⟩
+    | .beq    => ⟨[.nat, .nat], [], [.bool], .pure⟩
+    | .cst _  => ⟨[], [], [.nat], .pure⟩
 
 @[reducible]
 instance : DialectDenote Ex where
   denote
-    | .cst n, _, _ => n
-    | .add, .cons (a : Nat) (.cons b .nil), _ => a + b
-    | .beq, .cons (a : Nat) (.cons b .nil), _ => a == b
+    | .cst n, _, _ => n ::ₕ .nil
+    | .add, (a : Nat) ::ₕ b ::ₕ .nil, _ => a + b    ::ₕ .nil
+    | .beq, (a : Nat) ::ₕ b ::ₕ .nil, _ => (a == b) ::ₕ .nil
 
-def cst {Γ : Ctxt _} (n : ℕ) : Expr Ex Γ .pure .nat  :=
+def cst {Γ : Ctxt _} (n : ℕ) : Expr Ex Γ .pure [.nat] :=
   Expr.mk
     (op := .cst n)
     (ty_eq := rfl)
@@ -291,7 +314,7 @@ def cst {Γ : Ctxt _} (n : ℕ) : Expr Ex Γ .pure .nat  :=
     (args := .nil)
     (regArgs := .nil)
 
-def add {Γ : Ctxt _} (e₁ e₂ : Ctxt.Var Γ .nat) : Expr Ex Γ .pure .nat :=
+def add {Γ : Ctxt _} (e₁ e₂ : Ctxt.Var Γ .nat) : Expr Ex Γ .pure [.nat] :=
   Expr.mk
     (op := .add)
     (ty_eq := rfl)
@@ -301,20 +324,20 @@ def add {Γ : Ctxt _} (e₁ e₂ : Ctxt.Var Γ .nat) : Expr Ex Γ .pure .nat :=
 
 attribute [local simp] Ctxt.snoc
 
-def ex1_pre_dce : Com Ex ∅ .pure .nat :=
+def ex1_pre_dce : Com Ex ∅ .pure [.nat] :=
   Com.var (cst 1) <|
   Com.var (cst 2) <|
-  Com.ret ⟨0, by simp [Ctxt.snoc]⟩
+  Com.ret <| (⟨0, rfl⟩) ::ₕ .nil
 
-/-- TODO: how do we evaluate 'ex1_post_dce' within Lean? :D -/
-def ex1_post_dce : Com Ex ∅ .pure .nat := (dce' ex1_pre_dce).val
+def ex1_post_dce : Com Ex ∅ .pure [.nat] := (dce' ex1_pre_dce).val
 
-def ex1_post_dce_expected : Com Ex ∅ .pure .nat :=
+def ex1_post_dce_expected : Com Ex ∅ .pure [.nat] :=
   Com.var (cst 2) <|
-  Com.ret ⟨0, by simp [Ctxt.snoc]⟩
+  Com.ret <| (⟨0, rfl⟩) ::ₕ .nil
 
-theorem checkDCEasExpected :
-  ex1_post_dce = ex1_post_dce_expected := by native_decide
+-- TODO: uncomment once sorries are fixed
+-- theorem checkDCEasExpected :
+--   ex1_post_dce = ex1_post_dce_expected := by native_decide
 
 end Examples
 end DCE
