SSA/Core/Framework/ToExpr.lean
@@ -83,7 +83,7 @@ def mapVar {Γ : Ctxt d.Ty} (v : Γ.Var ty) : Q(Ctxt.Var $(f.mapCtxt Γ) $(f.map
   let i := toExpr v.1
   Ctxt.mkVar Ty Γ ty i none
 
-def mapArgs {Γ : Ctxt d.Ty} {argSig} (args : HVector (Γ.Var) argSig) :
+def mapVarVec {Γ : Ctxt d.Ty} {argSig} (args : HVector (Γ.Var) argSig) :
     Lean.Expr :=
   let Ty : Q(Type) := q(($d').Ty)
   let Γ := f.mapCtxt Γ
@@ -101,25 +101,25 @@ variable {d'} (f : DialectMetaMorphism d d')
   (dE : Q(Dialect)) (sig : Q(DialectSignature $dE)) in
 mutual
 
-partial def Com.toExprAux {Γ : Ctxt d.Ty} {eff : EffectKind} {ty : d.Ty}
+partial def Com.toExprAux {Γ : Ctxt d.Ty} {eff : EffectKind} {ty}
     (com : Com d Γ eff ty) : Lean.Expr :=
   let ΓE : Q(Ctxt ($dE).Ty) := f.mapCtxt Γ
-  let tyE : Q(($dE).Ty) := f.mapTy ty
+  let tyE : Q(List ($dE).Ty) := f.mapList ty
   let effE : Q(EffectKind) := Lean.toExpr eff
   match com with
-  | .ret v =>
-    let v := f.mapVar v
-    mkAppN (mkConst ``Com.ret) #[dE, sig, ΓE, tyE, effE, v]
-  | .var (α := eTy) e body =>
-    let eTyE := f.mapTy eTy
+  | .ret vs =>
+    let vs := f.mapVarVec vs
+    mkAppN (mkConst ``Com.ret) #[dE, sig, ΓE, tyE, effE, vs]
+  | .var (ty := eTy) e body =>
+    let eTyE := f.mapList eTy
     let e := e.toExprAux
     let body := body.toExprAux
     mkAppN (mkConst ``Com.var) #[dE, sig, ΓE, effE, eTyE, tyE, e, body]
 
-partial def Expr.toExprAux {Γ : Ctxt d.Ty} {eff : EffectKind} {ty : d.Ty} :
+partial def Expr.toExprAux {Γ : Ctxt d.Ty} {eff : EffectKind} {ty} :
     Expr d Γ eff ty → Lean.Expr :=
   let ΓE : Q(Ctxt ($dE).Ty) := f.mapCtxt Γ
-  let tyE : Q(($dE).Ty) := f.mapTy ty
+  let tyE : Q(($dE).Ty) := f.mapList ty
   let effE : Q(EffectKind) := Lean.toExpr eff
   fun
   | ⟨op, _ty_eq, eff_le, args, regArgs⟩ =>
@@ -128,24 +128,24 @@ partial def Expr.toExprAux {Γ : Ctxt d.Ty} {eff : EffectKind} {ty : d.Ty} :
     let ty_eq : Lean.Expr := mkApp2 (.const ``rfl [1]) Ty tyE
     let eff_le := f.mapEffLe eff_le
 
-    let args := f.mapArgs args
+    let args := f.mapVarVec args
     let regArgs := Regions.toExprAux regArgs
 
     mkAppN (mkConst ``Expr.mk) #[
       dE, sig, effE, ΓE, tyE, op, ty_eq, eff_le, args, regArgs
     ]
 
-partial def Regions.toExprAux {regSig : List (Ctxt d.Ty × d.Ty)}
+partial def Regions.toExprAux {regSig : RegionSignature d.Ty}
     (regs : HVector (fun (t : _ × _) => Com d t.1 EffectKind.impure t.2) regSig) :
     Lean.Expr :=
   let α := q(Ctxt ($dE).Ty × ($dE).Ty)
   let A :=
-    q(fun (t : Ctxt ($dE).Ty × ($dE).Ty) => Com $dE t.1 EffectKind.impure t.2)
+    q(fun (t : Ctxt ($dE).Ty × List ($dE).Ty) => Com $dE t.1 EffectKind.impure t.2)
   match regSig, regs with
   | [], .nil =>
     mkApp2 (.const ``HVector.nil [0,0]) α A
   | a::as, .cons x xs =>
-    let pToExpr (a) := Prod.foldToExpr <| a.map f.mapCtxt f.mapTy
+    let pToExpr (a) := Prod.foldToExpr <| a.map f.mapCtxt f.mapList
     let a := pToExpr a
     let as := (as.map pToExpr).foldToExpr
 
@@ -155,12 +155,15 @@ partial def Regions.toExprAux {regSig : List (Ctxt d.Ty × d.Ty)}
 
 end
 
+
+
 variable {Γ : Ctxt d.Ty} {eff : EffectKind} {ty : d.Ty}
 
 /-!
 ## MetaMap helper
 -/
 section Map
+variable {ty : _}
 
 /-- Map a meta morphism over a LeanMLIR program, to obtain a (Lean) `Expr` representing
 the mapped program. -/
